% @author Shuning Zhang
% @date 2020-01-30
\documentclass[a4paper, 11pt]{ctexart}
\usepackage{amsfonts, amsmath, amssymb}
\usepackage{enumerate}
\usepackage[top=2cm, bottom=2cm, left=2.5cm, right=2.5cm]{geometry}
\usepackage{multicol}
\begin{document}
    \begin{enumerate}
        \item % 1
        \item % 2
        \item % 3
        \item % 4
            {\heiti 证明}\quad 令 $\beta_1 = \alpha_1 + \alpha_2$, $\beta_2 = \alpha_2 + \alpha_3$, $\beta_3 = \alpha_3 + \alpha_1$. $\beta_1$, $\beta_2$, $\beta_3$ 显然可以被 $\alpha_1$, $\alpha_2$, $\alpha_3$ 线性表示.
            另一方面, 有
            \begin{gather*}
                \alpha_1 = \frac{\beta_1 - \beta_2 + \beta_3}{2}, \\
                \alpha_2 = \frac{\beta_1 + \beta_2 - \beta_3}{2}, \\
                \alpha_3 = \frac{-\beta_1 + \beta_2 + \beta_3}{2}.
            \end{gather*}
            因此 $\alpha_1$, $\alpha_2$, $\alpha_3$ 与 $\beta_1$, $\beta_2$, $\beta_3$ 线性等价.
        \item % 5
            {\heiti 证明}\quad 取 $k_1$, $k_2$, $\cdots$, $k_s \in K$, 使
            \begin{align*}
                    & k_1\alpha_1 + k_2(\alpha_1 + \alpha_2) + \cdots + k_s(\alpha_1 + \alpha_2 + \cdots + \alpha_s) \\
                ={} & (k_1 + k_2 + \cdots + k_s)\alpha_1 + (k_2 + \cdots + k_s)\alpha_2 + \cdots + k_s\alpha_s \\
                ={} & 0.    
            \end{align*}
            因为 $\alpha_1$, $\alpha_2$, $\cdots$, $\alpha_s$ 线性无关, 所以 $k_1 + k_2 + \cdots + k_s = k_2 + \cdots + k_s = \cdots = k_s = 0$,
            即 $k_1 = k_2 = \cdots = k_s = 0$. 因此 $\alpha_1$, $\alpha_1 + \alpha_2$, $\cdots$, $\alpha_1 + \alpha_2 + \cdots + \alpha_s$ 线性无关.
        \item % 6
            {\heiti 证明}\quad 取 $k_1$, $k_2$, $\cdots$, $k_s$, $k_{s+1} \in K$, 使
            \[
                k_1\alpha_1 + k_2\alpha_2 + \cdots + k_s\alpha_s + k_{s+1}\beta = 0,    
            \]
            若 $k_{s+1} = 0$, 则 $\alpha_1$, $\alpha_2$, $\cdots$, $\alpha_s$, $\beta$ 线性无关, 与题意相悖. 因此 $k_{s+1} \neq 0$, 即
            \[
                \beta = \frac{k_1}{k_{s+1}}\alpha_1 + \frac{k_2}{k_{s+1}}\alpha_2 + \cdots + \frac{k_s}{k_{s+1}}\alpha_s.    
            \]
        \item % 7
            略.
        \item % 8
            略.
        \item % 9
        \item % 10
        \item % 11
            略.
        \item % 12
        \item % 13
        \item % 14
        \item % 15
        \item % 16
        \item % 17
        \item % 18
        \item % 19
        \item % 20
        \item % 21
        \item % 22
        \item % 23
        \item % 24
        \item % 25
    \end{enumerate}
\end{document}
